changes after discussion

Core.v
@@ -9,29 +9,42 @@ Require Import DecidableType.
 Require Import Coq.Bool.Sumbool.
 Require Import Coq.Arith.Peano_dec.
 Require Import Coq.Relations.Relations.
-Require Import Setoid.
-
 
 Module Solver.
 
-Parameter flavor : Type.
-Parameter eq_flavor_dec : forall (f1 f2 : flavor), { f1 = f2 } + { ~ f1 = f2 }.
+(* Start with assumptions about flavors. Flavor equality is just Coq 
+   equality, but it is decidable.  We can also decide whether one 
+   flavor can rewrite another.  I'm using "sumbool" for the result of 
+   these two decision procedures. *)
+
+Parameter flavor : Set.
+Parameter eq_flavor_dec : forall (f1 f2 : flavor), 
+  { f1 = f2 } + { ~ f1 = f2 }.
+
+(* There are only a finite number of flavors, and we can list 
+   them all out. *)
+Parameter flavors : exists (l : list flavor), forall f : flavor, In f l.
+
 
 Parameter canRewrite : relation flavor.
 Notation "f1 >= f2" := (canRewrite f1 f2).
 Parameter canRewrite_dec : forall f1 f2, { f1 >= f2 } + { ~ f1 >= f2 }.
 
 Axiom R1 : transitive flavor canRewrite.
-Axiom R2 : forall f f1 f2, f1 >= f -> f2 >= f -> 
-    { f1 >= f2 } + { f2 >= f1 }.
-(* We don't have any useless flavors. 
-   Everything can be used for rewriting something. *)
+Axiom R2 : forall f f1 f2, 
+    f1 >= f -> f2 >= f -> f1 >= f2 \/ f2 >= f1.
+(* An extra axiom about flavors: We don't have any useless flavors. 
+   Everything can be used for rewriting something.... *)
+(* NOTE: Wanteds is a counter-example!!! *)
 Axiom R3 : forall f, exists f', f >= f'.
 
+(* If f rewrites anything, then it rewrites itself. *)
+Lemma SelfRewrite : forall f,  (exists f1, f >= f1) -> f >= f.
+intros. destruct H as [f1 H].
+pose (K := @R2 f1 f f H H). clearbody K. tauto.
+Qed.
 
 Definition var := nat.
-Module VarSet := MSetWeakList.Make Nat_as_OT.
-Module VarSetDecide := WDecideOn Nat_as_OT VarSet.
 
 Inductive ty : Set :=
   | tycon : ty
@@ -42,6 +55,9 @@ Definition eq_ty_dec : forall t1 t2 : ty, {t1 = t2} + {t1 <> t2}.
   intros; decide equality. apply eq_nat_dec.
 Qed.
 
+Module VarSet       := MSetWeakList.Make Nat_as_OT.
+Module VarSetDecide := WDecideOn Nat_as_OT VarSet.
+
 Fixpoint vars (t : ty) : VarSet.t :=
   match t with 
   | tycon => VarSet.empty
@@ -49,30 +65,42 @@ Fixpoint vars (t : ty) : VarSet.t :=
   | tyapp t1 t2 => VarSet.union (vars t1) (vars t2)
   end.
 
-Definition elt := (var * flavor * ty).
-Definition Subst := list elt.
+Definition elt : Set := (var * flavor * ty).
+Definition Subst : Set := list elt.
+(* Working from the picture of the whiteboard. *)
+
+(* This allows (a,f,t1) (a,f,t2) when not f >= f. 
+    (i.e. 2 wanteds that don't.) *)
 Definition WF1 (s : Subst) := forall a f1 t1 f2 t2,  
      In (a, f1, t1) s -> In (a, f2, t2) s -> 
      t1 <> t2 -> not (f1 >= f2).
 
 Definition WF2 (s : Subst) := forall a f, 
   not (In (a, f, tyvar a) s).
+
 Definition noids (s : Subst) := WF2 s.
 
+(* This was on the board, but I don't think it is true. 
+   What if f can't rewrite itself? *)
 Lemma L1 : forall s (f : flavor) a t1 t2, 
-  WF1 s -> In (a, f, t1) s -> In (a, f, t2) s -> t1 = t2.
+  WF1 s -> f >= f -> In (a, f, t1) s -> In (a, f, t2) s -> t1 = t2.
 Proof.  intros. 
   destruct (eq_ty_dec t1 t2) as [Y | N]. exact Y. 
-  pose (J := H _ _ _ _ _ H0 H1 N).
-Admitted.
-(* I don't think this is true. what if f can't rewrite itself? *)
+  pose (J := H _ _ _ _ _ H1 H2 N). clearbody J.
+  contradiction.
+Qed.
 
-(* Lookup the first tuple in the list that works. *)
+
+(* A very concrete definition of applying the substition. 
+   We just lookup the first tuple in the list that works.
+   (Is this what GHC does?) *)
 Fixpoint apply (s : Subst) (f : flavor) (a : var) : option ty := 
   match s with 
   | nil => None
   | (a1,f1,t1) :: s' => 
-     if sumbool_and _ _ _ _ (eq_nat_dec a a1) (canRewrite_dec f1 f)
+     if sumbool_and _ _ _ _ 
+        (eq_nat_dec a a1) 
+        (canRewrite_dec f1 f)
      then Some t1 else apply s' f a 
   end.
 
@@ -81,14 +109,16 @@ Lemma WF1_tail : forall a f t s, WF1 ((a,f,t)::s) -> WF1 s.
   right. auto. right. auto. auto.
 Qed.
 
-(* It doesn't necessarily have to be the first tuple. *)
+(* Here's an alternative to L1.  
+   It doesn't necessarily have to be the first tuple. *)
 Lemma apply_in : forall s f f1 a t, 
   WF1 s -> In (a, f1, t) s -> f1 >= f -> apply s f a = Some t.
  intros. 
  induction s. inversion H0.
  destruct a0 as [[a2 f2] t2]. simpl.
  destruct (eq_nat_dec a a2); destruct (canRewrite_dec f2 f); simpl.
- - subst. destruct (eq_ty_dec t2 t). f_equal. auto.
+ - subst. 
+   destruct (eq_ty_dec t2 t). f_equal. auto.
    inversion H0. inversion H2. rewrite H5 in n. tauto. (* n <> n *)
    assert (I : In (a2, f2, t2) ((a2,f2,t2) :: s)). simpl. left. auto.
    destruct (R2 H1 c).
@@ -104,6 +134,24 @@ Lemma apply_in : forall s f f1 a t,
    apply IHs. eapply WF1_tail. eauto. auto.
 Qed.  
 
+(* We can also invert the function. *)
+Lemma in_apply : forall s f a t, 
+  apply s f a = Some t -> exists f1, f1 >= f /\ In (a, f1, t) s.
+  induction s; intros; simpl in H. inversion H.
+  destruct a as [p0 t1]. destruct p0 as [a1 f1].
+  destruct (eq_nat_dec a0 a1); destruct (canRewrite_dec f1 f); simpl in H.
+  - inversion H. exists f1. split. auto. subst. simpl. left. auto.
+  - subst. destruct (IHs f a1 t H) as [f2 [J K]].
+    exists f2. split. auto. simpl. right. auto.
+  - subst. destruct (IHs f a0 t H) as [f2 [J K]].
+    exists f2. split. auto. simpl. right. auto.
+  - subst. destruct (IHs f a0 t H) as [f2 [J K]].
+    exists f2. split. auto. simpl. right. auto.
+Qed.
+   
+
+(* Extend the substitution to types *)
+
 Fixpoint apply_ty (s : Subst) (f : flavor) (t : ty) : ty :=
   match t with 
   | tycon => tycon
@@ -114,51 +162,262 @@ Fixpoint apply_ty (s : Subst) (f : flavor) (t : ty) : ty :=
   | tyapp t1 t2 => tyapp (apply_ty s f t1) (apply_ty s f t2)
   end.
 
-Definition selfapp (s : Subst) (f : flavor) : Subst := 
-  map (fun e => 
-   match e with 
-    | (a,f1, t) => (a, f1, apply_ty s f t)
-   end) s.
+(* This is from the triangular substitutions paper. 
+   Define a substituion to be well formed if there are 
+   no cycles. 
+ *)
 
-Definition tri s f y x := 
-    match apply s f x with 
+(* is y connected to x through some rewrite. *)
+Definition tri s y x := 
+  exists f, match apply s f x with 
     | Some t => VarSet.In y (vars t)
     | None => False
     end.
 
-(* From Triangular substitutions paper. *)
-
 Definition wfs (s : Subst) := 
-  forall a f, not ((clos_trans _ (tri s f)) a a). 
+  forall (a : var), not ((clos_trans var (tri s)) a a). 
 
 Lemma wfs_noids : forall s, WF1 s -> wfs s -> noids s.
   intros s H1 H. unfold noids. unfold WF2. unfold not. intros.
   unfold wfs in H. unfold not in H.
-  destruct (R3 f) as [f' Hf']. apply (H a f').
+  destruct (R3 f) as [f' Hf']. apply (H a).
   apply t_step. assert (apply s f' a = Some (tyvar a)).
   eapply apply_in. eauto. eauto. eauto. 
-  unfold tri. rewrite H2. simpl. 
+  unfold tri. exists f'. rewrite H2. simpl. 
+  (* This is a general purpose tactic from the MSets library
+  for proving facts about finite sets. *)
   VarSetDecide.fsetdec.
 Qed.
 
-Lemma wfs_selfapp : forall s f, WF1 s -> wfs s <-> wfs (selfapp s f).
+Lemma var_in_union : forall a s1 s2, VarSet.In a (VarSet.union s1 s2) -> 
+  VarSet.In a s1 \/ VarSet.In a s2.
+intros. VarSetDecide.fsetdec.
+Qed. 
+
+Lemma vars_in_apply_ty : forall s a f t, 
+  VarSet.In a (vars (apply_ty s f t)) -> 
+  VarSet.In a (vars t) \/ exists b t0,  
+    VarSet.In a (vars t0) /\ apply s f b = Some t0 /\ VarSet.In b (vars t).
+induction t; intros; simpl in H. 
+  - inversion H.
+  - destruct (eq_nat_dec a v). subst. left. simpl. VarSetDecide.fsetdec.
+    right. exists v. destruct (apply s f v). exists t. simpl. split; auto.
+       split. auto. VarSetDecide.fsetdec.
+    simpl in H. VarSetDecide.fsetdec.
+  - destruct (var_in_union H) as [L | R].
+     destruct (IHt1 L) as [M | [b [t0 [In [Ap Inb]]]]]. left. simpl. VarSetDecide.fsetdec.
+       right. exists b. exists t0. simpl. split. auto. split. auto. VarSetDecide.fsetdec.
+     destruct (IHt2 R) as [M | [b [t0 [In [Ap Inb]]]]]. left. simpl. VarSetDecide.fsetdec.
+       right. exists b. exists t0. simpl. split. auto. split. auto. VarSetDecide.fsetdec.
+Qed.
+
+(* ?????   
+  Do we need to check the interaction between f and f1 in 
+  the self application?   *)
+Definition apply_e s f (e : elt) : elt := 
+  match e with
+  | (a, f1, t) => 
+    if canRewrite_dec f f1 then 
+      (a, f1, apply_ty s f t)
+    else
+      (a, f1, t)
+  end.
+
+(* The first result of the triangular substitutions paper. *)
+Definition selfapp (s : Subst) (f : flavor) : Subst := 
+  map (apply_e s f) s.
+
+Definition map_option A B (f: A -> B) o := 
+  match o with 
+  | Some t => Some (f t)
+  | None   => None
+  end.
+
+Lemma map_apply : forall s1 f1 s f y o,
+   apply s f y = o -> 
+   apply (map (apply_e s1 f1) s) f y = map_option (apply_ty s1 f1) o.
+destruct o.
+induction s. intros. inversion H. 
+intros. destruct a as [[a0 f0] t0].
+simpl. simpl in H. 
+destruct (eq_nat_dec y a0);
+destruct (canRewrite_dec f0 f). 
+- simpl. subst. simpl in H. inversion H. auto.
+- simpl. subst. simpl in H. apply IHs. auto.
+- simpl. subst. simpl in H. apply IHs. auto.
+- simpl. subst. simpl in H. apply IHs. auto.
+- intros. simpl.
 Admitted.
 
+
+(* If a var is free in S_f (t) then either it was in t, or it is in 
+   some b that was substituted in t.*)
+Lemma in_apply_ty : forall a s f t,
+VarSet.In a (vars  (apply_ty s f t)) -> VarSet.In a (vars t) \/ 
+  exists b t0, VarSet.In b (vars t) /\ apply s f b = Some t0 /\ VarSet.In a (vars t0).
+induction t; intros.
+- simpl in H. VarSetDecide.fsetdec.
+- simpl in *. 
+  case_eq (apply s f v); intros. rewrite H0 in H.
+    right. exists v. exists t. split. VarSetDecide.fsetdec. tauto.
+    rewrite H0 in H. simpl in H. inversion H. subst. left. auto.
+       subst. inversion H2.
+- simpl in *.
+  destruct (var_in_union H) as [L | R].
+    destruct (IHt1 L) as [ In | [b [t0 [M [N P]]]]].
+    VarSetDecide.fsetdec.
+    right. exists b. exists t0. split. VarSetDecide.fsetdec. tauto.
+    destruct (IHt2 R) as [ In | [b [t0 [M [N P]]]]].
+    VarSetDecide.fsetdec.
+    right. exists b. exists t0. split. VarSetDecide.fsetdec. tauto.
+Qed.
+
+(* If you can get there taking two steps at a time, you 
+  can get there taking one step at a time. *)
+Lemma step: forall s f a y,
+  clos_trans var (tri (selfapp s f)) a y -> 
+  clos_trans var (tri s) a y.
+intros. induction H; subst.
+(* single step case *)
+- unfold selfapp, tri in H.
+  destruct H as [f0 M].
+  case_eq (apply s f0 y); intros.
+  assert (H1 : apply (map (apply_e s f) s) f0 y =
+               map_option (apply_ty s f) (Some t)). eapply map_apply; eauto.
+  rewrite H1 in M.
+  destruct (in_apply_ty _ _ _ M).
+    apply t_step. unfold tri. exists f0. rewrite H. auto.
+    destruct H0 as [b [t0 [N [P Q]]]].
+    apply t_trans with (y := b). 
+      apply t_step. unfold tri. exists f. rewrite P. auto.
+      apply t_step. unfold tri. exists f0. rewrite H. auto.
+  pose (K:= map_apply s f _ _ _ H). simpl in K.
+  rewrite K in M. contradiction.
+- apply t_trans with (y := y). auto. auto.
+Qed.
+
+(* If you can get there taking one at a time, you 
+  can get there taking two steps at a time. *)
+(* Probably not true *)
+(*
+Lemma step_two_one : forall s f a y,
+  clos_trans var (tri s) a y -> 
+  clos_trans var (tri (selfapp s f)) a y.
+intros. induction H; unfold tri in H.
+- destruct H as [f0 M].
+case_eq (apply s f0 y); intros; rewrite H in M.
+apply t_step. unfold tri. exists f0. unfold selfapp.
+apply map_apply with (s := s) (f := f0)(s1:= s)(f1:=f) in H.
+rewrite H. simpl. admit. 
+contradiction.
+- apply t_trans with (y := y). auto. auto.
+Qed.
+*)
+
+Lemma wfs_selfapp : forall s f, WF1 s -> wfs s <-> wfs (selfapp s f).
+intros. split.
+(* left to right*)
+- unfold wfs. unfold not. intros H1 a CT. apply (H1 a).
+  inversion CT. subst. unfold tri in H0. destruct H0 as [f0 H0].
+  assert (EQ : exists t, apply (selfapp s f) f0 a = Some t).
+  destruct (apply (selfapp s f) f0 a). exists t. auto. inversion H0.
+  destruct EQ as [t EQ].
+  rewrite EQ in H0.
+  destruct (in_apply _ _ _ EQ) as [f1 [J K]].
+  unfold selfapp in K.
+  rewrite in_map_iff in K. destruct K as [[[a0 f3] t0] [L M]].
+  inversion L. subst. clear L.
+  assert (apply s f0 a = Some t0). eapply apply_in; eauto.
+  destruct (vars_in_apply_ty _ _ _ H0) as [N | [b [t1 [In [Ap Inb]]]]].
+  eapply t_step. unfold tri. exists f0. rewrite H2. auto. 
+  apply t_trans with (y := b). apply t_step. unfold tri.
+  exists f. rewrite Ap. auto. apply t_step. unfold tri.
+  exists f0. rewrite H2. auto. 
+  subst. apply (step _ _ CT).
+(* right to left *)
+- unfold wfs, not. intros H1 a CT. apply (H1 a).
+inversion CT. subst. unfold tri in H0. destruct H0 as [f0 H0].
+  (* Kinda stuck *)
+Admitted.
+
+
+(* It's not clear to me which version of the iterated substitution is 
+   easier to work with. *)
+
+(* Apply a substitution to itself n times. *)
+Definition selfapp_n (n : nat) (s : Subst) (f : flavor) : Subst :=
+  nat_rec (fun _ => Subst) s (fun _ =>  map (apply_e s f)) n.
+
+Lemma selfapp_once : forall s f,
+  selfapp_n (S 0) f s = selfapp f s.
+intros. simpl. unfold selfapp. auto.
+Qed.
+
+Lemma selfapp_many : forall s f n,
+  selfapp_n (S n) s f = map (apply_e s f) (selfapp_n n s f).
+intros. simpl. unfold selfapp. auto.
+Qed.
+
+(* Apply a substitution to a ty n times *)
 Fixpoint apply_n (n : nat) (s : Subst) (f : flavor) (t : ty) : ty := 
   match n with 
   | 0 => t
   | S m => apply_ty s f (apply_n m s f t)
   end.
 
+Lemma apply_n_tycon : forall n s f, apply_n n s f tycon = tycon.
+induction n. intros. simpl. auto.
+intros. simpl. rewrite IHn. simpl. auto.
+Qed.
 
-Definition IG1 s := forall f t, 
-      exists n, apply_n n s f t = apply_n (S n) s f t.
+Lemma apply_n_app : forall n s f t1 t2, 
+  apply_n n s f (tyapp t1 t2) = 
+  tyapp (apply_n n s f t1) (apply_n n s f t2).
+induction n; intros; simpl; auto.
+rewrite IHn. simpl. auto.
+Qed.
 
-(* I don't believe this. The n could depend on t, and there are an infinite number of these. 
-Axiom IG1C : exists n, forall s f t, apply_n n s f t = apply_n (S n) s f t. *)
 
-Lemma L2 : forall s s', IG1 s -> incl s' s ->  IG1 s'.
+Lemma iterate : forall n s f t, 
+  apply_ty (selfapp_n n s f) f t = apply_n (S n) s f t.
+induction n; intros.
+  - simpl. auto.
+  - simpl in IHn. simpl. rewrite <- IHn.
+(* STUCK *)
+Admitted.
+
+Definition IG1 s := 
+  forall f t, 
+    exists n, apply_n n s f t = apply_n (S n) s f t.
+
+Definition IG1C s := exists n, 
+  forall f t, 
+    apply_n n s f t = apply_n (S n) s f t.
+
+
+Lemma one_n : forall s, IG1 s -> IG1C s.
+(* I don't believe this. The n *could* depend on t, 
+    and there are an infinite number of these. *)
+Admitted.
+
+Definition IG1A s := forall f, 
+      exists n, selfapp_n n s f = selfapp_n (S n) s f.
+Definition IG1AC s := exists n, forall f, 
+      selfapp_n n s f = selfapp_n (S n) s f.
+Lemma one_nA : forall s, IG1A s -> IG1AC s.
+intros.
+unfold IG1A,IG1AC in *.  destruct flavors as [l F].
 Admitted.
 
 
+
+Lemma L2 : forall s s', IG1 s -> incl s' s ->  IG1 s'.
+unfold incl, IG1. intros.
+destruct (H f t) as [n K].
+exists n.
+induction t. simpl. rewrite apply_n_tycon. simpl. auto.
+simpl. 
+Admitted.
+
+Lemma fixpoint : forall s, WF1 s -> wfs s <-> IG1 s.
 
